added to dev.thy a proof that if you only write non-empty blocks, all the blocks that you read will be non-empty.  Also substantially rewrote README.md with many more details

dev.thy
@@ -31,14 +31,49 @@ lemma initial_block_size :
   (* proof by sledgehammer cvc5 zipperposition vampire verit *)
   by (simp add: init_block_size initial_dev_def)
 
+lemma initial_dev_never_null :
+"initial_dev (Suc bs) index \<noteq> Nil"
+  by (simp add: initial_dev_def)
+
 fun write_block :: "dev \<Rightarrow> nat \<Rightarrow> data_block \<Rightarrow> dev" where
 "write_block dev bn data = (\<lambda> index . (if index = bn then data else dev index))"
 
-(* true, but not needed for our theorem
+(* true, but not needed for our theorem *)
 lemma read_block_returns_immediately_written :
 "(write_block dev bn data) bn = data"
   by simp
+
+(* bbs is a list of pairs of block numbers and blocks *)
+fun write_all :: "dev \<Rightarrow> (nat * data_block) list \<Rightarrow> dev" where
+"write_all dev [] = dev" |
+"write_all dev ((bn, block) # bbs) =
+   write_block (write_all dev bbs) bn block"
+
+lemma write_all_empty : "write_all dev [] = dev"
+  by simp
+(*
+lemma write_all_single :
+"write_all dev [(bn, block)] = write_block dev bn block"
+  by simp
+
+lemma write_all_induct :
+"write_all dev ((bn, block) # bbs) =
+ write_block (write_all dev bbs) bn block"
+  by simp
 *)
+
+(* if we only write non-empty blocks, we will only read non-empty blocks
+   Suc bs is a block size > 0 *)
+lemma write_nonempty_blocks :
+"(\<forall> (bn, block) \<in> set bbs . length block = (Suc bs)) \<Longrightarrow>
+  write_all (initial_dev (Suc bs)) bbs bn \<noteq> Nil"
+  apply (induct bbs arbitrary: bn dev)
+  using initial_dev_never_null write_all_empty
+  apply (presburger)
+  by (smt (verit, ccfv_threshold) list.distinct(1)
+      list.inject list.set_intros(1,2) list.size(3)
+      old.nat.distinct(1) old.prod.case
+      write_all.elims write_block.simps)
 
 (* function to demonstrate that even if we write any and all,
    except as long as we avoid the given block number/bn,
@@ -83,9 +118,15 @@ proof (induct writes)
   then show ?case using initial_block_size by simp
 next
   case (Cons a writes)
-  then show ?case  (* proof found by sledgehammer cvc5 *)
+  then show ?case  (* proof found by sledgehammer cvc5, and another by e *)
     by (smt (verit) initial_block_size list.inject write_block.simps
         write_same_sized_blocks.elims)
 qed
+
+fun all_blocks :: "nat \<Rightarrow> nat \<Rightarrow> dev \<Rightarrow> data_block list" where
+"all_blocks from 0 dev = []" |
+"all_blocks from nb dev = (dev from) # (all_blocks (from + 1) (nb - 1) dev)"
+
+value "all_blocks 0 3 (initial_dev 4)"
 
 end
