README.md
@@ -1,5 +1,44 @@
-The goal of this project is to create a provably correct file system
-implementation that is also efficient.
+This is a project to design, implement, and formally prove correctness
+of file system code.  The ultimate goal of this project is to create a
+provably correct file system implementation that is also efficient.
 
 Code correctness is proven with the Isabelle 2025 theorem prover,
   https://isabelle.in.tum.de/website-Isabelle2025/
+
+The first two designs are for a RAM-based file system, where the
+data is stored in memory.  The file system is a list of pairs,
+where the first element of a pair is the file name and the second
+is the file contents.
+
+A write in ramfs_unlimited always succeeds, possibly overwriting a
+pre-existing file with the same name.
+
+A write in ramfs_sized may fail if either the file system already
+has a file with the given name, or the amount of space in the
+file system is insufficient to accomodate the given file.
+
+Interesting proofs in ramfs_sized are identified with the word "theorem"
+(as opposed to the word "lemma").  They include
+
+1. the code preserving file name uniqueness (write_preserves_distinct
+and remove_preserves_distinct),
+
+2. a file that can be read once remains unchanged as long as it is not
+explicitly removed (multiple_op_preserves_read), and
+
+3. a file can only be created through a write of the given name
+(multiple_op_name_not_created).
+
+Moving on from files stored in memory, persistent file systems write
+data to a disk device.  This functionality is given by dev.thy, which
+includes the type "dev", a function from block numbers to block contents,
+and the function "write_block", which given a device, a block number,
+and block contents, returns a new device that will return the given
+block contents for the given block
+number.
+
+Current work includes developing a file system that uses dev.thy and that
+is provably correct and as simple as possible.  A goal of future work
+will be an efficient and provably correct file system, perhaps also crash
+resistant. The Linux B-Tree file system (BTRFS) will likely be used as
+inspiration.
